Removed Fence and Observe, added ExtPut and ExtGet: theory/bir now compiles

src/theory/bir/HolBACoreSimps.sml
@@ -27,14 +27,14 @@ val bir_list_of_types = [
    mk_thy_type {Tyop="bir_label_t",          Thy="bir_program", Args=[]},
    mk_thy_type {Tyop="bir_label_exp_t",      Thy="bir_program", Args=[]},
    mk_thy_type {Tyop="bir_stmt_end_t",       Thy="bir_program", Args=[]},
-   mk_thy_type {Tyop="bir_stmt_basic_t",     Thy="bir_program", Args=[Type.alpha]},
+   mk_thy_type {Tyop="bir_stmt_basic_t",     Thy="bir_program", Args=[]},
    mk_thy_type {Tyop="bmc_stmt_basic_t",     Thy="bir_program", Args=[]},
    mk_thy_type {Tyop="bir_generic_stmt_t",   Thy="bir_program", Args=[Type.alpha]},
    mk_thy_type {Tyop="bir_generic_block_t",  Thy="bir_program", Args=[Type.alpha]},
    mk_thy_type {Tyop="bir_generic_program_t",Thy="bir_program", Args=[Type.alpha]},
    mk_thy_type {Tyop="bir_programcounter_t", Thy="bir_program", Args=[]},
    mk_thy_type {Tyop="bir_status_t",         Thy="bir_program", Args=[]},
-   mk_thy_type {Tyop="bir_inflight_stmt_t",  Thy="bir_program", Args=[Type.alpha]},
+   mk_thy_type {Tyop="bir_inflight_stmt_t",  Thy="bir_program", Args=[]},
    mk_thy_type {Tyop="bir_state_t",          Thy="bir_program", Args=[]},
    mk_thy_type {Tyop="bir_execution_result_t", Thy="bir_program", Args=[Type.alpha]}
 ];
