src/theory/bir/bir_expScript.sml
@@ -28,13 +28,13 @@ val _ = Datatype `bir_exp_t =
 
   | BExp_IfThenElse        bir_exp_t bir_exp_t bir_exp_t
 
-  (* TODO: The get function could also take a BIR state, but this is only defined later *)
-  | BExp_ExtGet            ('ext_state_t -> bir_val_t option) bir_type_t
+  | BExp_ExtGet            string bir_type_t (* string should map to a ('ext_state_t -> bir_val_t option) somewhere *)
+
   | BExp_Load              bir_exp_t bir_exp_t bir_endian_t bir_immtype_t
   | BExp_Store             bir_exp_t bir_exp_t bir_endian_t bir_exp_t
-(*  | BExp_TAS               bir_exp_t bir_exp_t bir_endian_t bir_exp_t bir_exp_t *)
-                           `;
+`;
 
+(* TODO: Update these? Or use bir_vars_of_exp instead? *)
 val _ = Datatype `bir_exp_algebra_t =
   <| bexp_const : bir_imm_t -> 'carrier_t;
      bexp_memconst : bir_immtype_t -> bir_immtype_t -> (num |-> num) -> 'carrier_t;
@@ -177,6 +177,15 @@ val bir_eval_ifthenelse_def = Define `
        if (cw = 1w) then SOME v1 else SOME v2) /\
   (bir_eval_ifthenelse _ _ _ = NONE)`;
 
+val bir_eval_extget_def = Define `
+  (bir_eval_extget ext_map ext_name ty =
+    case FLOOKUP (FST ext_map) ext_name of
+    | SOME v =>
+      if type_of_bir_val v <> ty
+      then NONE
+      else SOME v
+    | NONE => NONE)`;
+
 val bir_eval_load_def = Define `
   (bir_eval_load (SOME (BVal_Mem ta tv mmap)) (SOME (BVal_Imm a)) en t =
      if ((type_of_bir_imm a) = ta) then
@@ -196,42 +205,41 @@ val bir_eval_store_def = Define `
   (bir_eval_store _ _ _ _ = NONE)`;
 
 
-
 val bir_eval_exp_def = Define `
-  (bir_eval_exp (BExp_Const n) env = SOME (BVal_Imm n)) /\
+  (bir_eval_exp ext_map (BExp_Const n) env ext_st = SOME (BVal_Imm n)) /\
 
-  (bir_eval_exp (BExp_MemConst aty vty mmap) env = SOME (BVal_Mem aty vty mmap)) /\
+  (bir_eval_exp ext_map (BExp_MemConst aty vty mmap) env ext_st = SOME (BVal_Mem aty vty mmap)) /\
 
-  (bir_eval_exp (BExp_Den v) env = bir_env_read v env) /\
+  (bir_eval_exp ext_map (BExp_Den v) env ext_st = bir_env_read v env) /\
 
-  (bir_eval_exp (BExp_Cast ct e ty) env = (
-     bir_eval_cast ct (bir_eval_exp e env) ty)) /\
+  (bir_eval_exp ext_map (BExp_Cast ct e ty) env ext_st = (
+     bir_eval_cast ct (bir_eval_exp ext_map e env ext_st) ty)) /\
 
-  (bir_eval_exp (BExp_UnaryExp et e) env = (
-     bir_eval_unary_exp et (bir_eval_exp e env))) /\
+  (bir_eval_exp ext_map (BExp_UnaryExp et e) env ext_st = (
+     bir_eval_unary_exp et (bir_eval_exp ext_map e env ext_st))) /\
 
-  (bir_eval_exp (BExp_BinExp et e1 e2) env = (
-     bir_eval_bin_exp et (bir_eval_exp e1 env) (bir_eval_exp e2 env))) /\
+  (bir_eval_exp ext_map (BExp_BinExp et e1 e2) env ext_st = (
+     bir_eval_bin_exp et (bir_eval_exp ext_map e1 env ext_st) (bir_eval_exp ext_map e2 env ext_st))) /\
 
-  (bir_eval_exp (BExp_BinPred pt e1 e2) env = (
-     bir_eval_bin_pred pt (bir_eval_exp e1 env) (bir_eval_exp e2 env))) /\
+  (bir_eval_exp ext_map (BExp_BinPred pt e1 e2) env ext_st = (
+     bir_eval_bin_pred pt (bir_eval_exp ext_map e1 env ext_st) (bir_eval_exp ext_map e2 env ext_st))) /\
 
-  (bir_eval_exp (BExp_MemEq e1 e2) env = (
-     bir_eval_memeq (bir_eval_exp e1 env) (bir_eval_exp e2 env))) /\
+  (bir_eval_exp ext_map (BExp_MemEq e1 e2) env ext_st = (
+     bir_eval_memeq (bir_eval_exp ext_map e1 env ext_st) (bir_eval_exp ext_map e2 env ext_st))) /\
 
-
-  (bir_eval_exp (BExp_IfThenElse c et ef) env =
-     bir_eval_ifthenelse (bir_eval_exp c env) (bir_eval_exp et env) (bir_eval_exp ef env)
+  (bir_eval_exp ext_map (BExp_IfThenElse c et ef) env ext_st =
+     bir_eval_ifthenelse (bir_eval_exp ext_map c env ext_st) (bir_eval_exp ext_map et env ext_st) (bir_eval_exp ext_map ef env ext_st)
   ) /\
 
-  (bir_eval_exp (BExp_Load mem_e a_e en ty) env =
-     bir_eval_load (bir_eval_exp mem_e env) (bir_eval_exp a_e env) en ty) /\
+  (bir_eval_exp ext_map (BExp_ExtGet ext_name ty) env ext_st =
+     bir_eval_extget ext_map ext_name ty) /\
 
-  (bir_eval_exp (BExp_Store mem_e a_e en v_e) env =
-     bir_eval_store (bir_eval_exp mem_e env) (bir_eval_exp a_e env) en (bir_eval_exp v_e env))
+  (bir_eval_exp ext_map (BExp_Load mem_e a_e en ty) env ext_st =
+     bir_eval_load (bir_eval_exp ext_map mem_e env ext_st) (bir_eval_exp ext_map a_e env ext_st) en ty) /\
+
+  (bir_eval_exp ext_map (BExp_Store mem_e a_e en v_e) env ext_st =
+     bir_eval_store (bir_eval_exp ext_map mem_e env ext_st) (bir_eval_exp ext_map a_e env ext_st) en (bir_eval_exp ext_map v_e env ext_st))
 `;
-
-
 
 
 (* ------------------------------------------------------------------------- *)
@@ -337,6 +345,10 @@ Cases_on `c` >> Cases_on `b` >> Cases_on `v` >> (
     bir_val_checker_REWRS]
 ));
 
+val bir_eval_extget_NONE_REWR = prove (
+  ``(!ext_put_map ext_name ty. bir_eval_extget (FEMPTY, ext_put_map) ext_name ty = NONE)``,
+
+fs [bir_eval_extget_def]);
 
 val bir_eval_load_NONE_REWRS1 = prove (
   ``(!mem en t. bir_eval_load mem NONE en t = NONE) /\
