src/theory/bir/bir_typing_expScript.sml
@@ -20,49 +20,54 @@ val bir_type_ss = rewrites (type_rws ``:bir_type_t``);
 
 
 val type_of_bir_exp_def = Define `
-  (type_of_bir_exp (BExp_Const i) = SOME (BType_Imm (type_of_bir_imm i))) /\
+  (type_of_bir_exp ext_map (BExp_Const i) = SOME (BType_Imm (type_of_bir_imm i))) /\
 
-  (type_of_bir_exp (BExp_MemConst aty vty mmap) = SOME (BType_Mem aty vty)) /\
+  (type_of_bir_exp ext_map (BExp_MemConst aty vty mmap) = SOME (BType_Mem aty vty)) /\
 
-  (type_of_bir_exp (BExp_Den v) = SOME (bir_var_type v)) /\
+  (type_of_bir_exp ext_map (BExp_Den v) = SOME (bir_var_type v)) /\
 
-  (type_of_bir_exp (BExp_Cast ct e rty) = (case (type_of_bir_exp e) of
+  (type_of_bir_exp ext_map (BExp_Cast ct e rty) = (case (type_of_bir_exp ext_map e) of
       NONE => NONE
     | SOME ty => (if (bir_type_is_Imm ty) then SOME (BType_Imm rty) else NONE))) /\
 
-  (type_of_bir_exp (BExp_UnaryExp et e) = (case (type_of_bir_exp e) of
+  (type_of_bir_exp ext_map (BExp_UnaryExp et e) = (case (type_of_bir_exp ext_map e) of
       NONE => NONE
     | SOME ty => (if (bir_type_is_Imm ty) then
         SOME ty else NONE))) /\
 
-  (type_of_bir_exp (BExp_BinExp et e1 e2) = (case (type_of_bir_exp e1,
-       type_of_bir_exp e2) of
+  (type_of_bir_exp ext_map (BExp_BinExp et e1 e2) = (case (type_of_bir_exp ext_map e1,
+       type_of_bir_exp ext_map e2) of
        (SOME ty1, SOME ty2) => (if ((bir_type_is_Imm ty1) /\ (ty2 = ty1)) then SOME ty1 else NONE)
        | _, _ => NONE)) /\
 
-  (type_of_bir_exp (BExp_BinPred pt e1 e2) = (case (type_of_bir_exp e1,
-       type_of_bir_exp e2) of
+  (type_of_bir_exp ext_map (BExp_BinPred pt e1 e2) = (case (type_of_bir_exp ext_map e1,
+       type_of_bir_exp ext_map e2) of
        (SOME ty1, SOME ty2) => (if ((bir_type_is_Imm ty1) /\ (ty2 = ty1)) then SOME BType_Bool else NONE)
        | _, _ => NONE)) /\
 
-  (type_of_bir_exp (BExp_MemEq e1 e2) = (case (type_of_bir_exp e1,
-       type_of_bir_exp e2) of
+  (type_of_bir_exp ext_map (BExp_MemEq e1 e2) = (case (type_of_bir_exp ext_map e1,
+       type_of_bir_exp ext_map e2) of
        (SOME (BType_Mem aty1 vty1), SOME (BType_Mem aty2 vty2)) => (if ((aty2 = aty1) /\ (vty2 = vty1)) then SOME BType_Bool else NONE)
        | _, _ => NONE)) /\
 
 
-  (type_of_bir_exp (BExp_IfThenElse ec e1 e2) = (case (type_of_bir_exp ec, type_of_bir_exp e1,
-       type_of_bir_exp e2) of
+  (type_of_bir_exp ext_map (BExp_IfThenElse ec e1 e2) = (case (type_of_bir_exp ext_map ec, type_of_bir_exp ext_map e1,
+       type_of_bir_exp ext_map e2) of
        (SOME ect, SOME ty1, SOME ty2) => (if ((ect = BType_Bool) /\ (ty2 = ty1)) then SOME ty1 else NONE)
        | _, _, _ => NONE)) /\
 
-  (type_of_bir_exp (BExp_Load me ae en rty) = (case (type_of_bir_exp me, type_of_bir_exp ae) of
+  (type_of_bir_exp ext_map (BExp_ExtGet ext_name ty) =
+    case FLOOKUP (FST ext_map) ext_name of
+    | SOME v => if type_of_bir_val v = ty then SOME ty else NONE
+    | NONE => NONE) /\
+
+  (type_of_bir_exp ext_map (BExp_Load me ae en rty) = (case (type_of_bir_exp ext_map me, type_of_bir_exp ext_map ae) of
        (SOME (BType_Mem aty vty), SOME (BType_Imm aty')) => (if (
             (aty = aty') /\ (if en = BEnd_NoEndian then (vty = rty) else (bir_number_of_mem_splits vty rty aty <> NONE))
            ) then SOME (BType_Imm rty) else NONE)
        | _, _ => NONE)) /\
 
-  (type_of_bir_exp (BExp_Store me ae en v) = (case (type_of_bir_exp me, type_of_bir_exp ae, type_of_bir_exp v) of
+  (type_of_bir_exp ext_map (BExp_Store me ae en v) = (case (type_of_bir_exp ext_map me, type_of_bir_exp ext_map ae, type_of_bir_exp ext_map v) of
        (SOME (BType_Mem aty vty), SOME (BType_Imm aty'), SOME (BType_Imm rty)) => (if (
             (aty = aty') /\ (if en = BEnd_NoEndian then (vty = rty) else (bir_number_of_mem_splits vty rty aty <> NONE))
            ) then SOME (BType_Mem aty vty) else NONE)
@@ -71,10 +76,11 @@ val type_of_bir_exp_def = Define `
 
 
 val type_of_bir_exp_THM = store_thm ("type_of_bir_exp_THM",
- ``!env e ty. (type_of_bir_exp e = SOME ty) ==>
-              ((bir_eval_exp e env = NONE) \/ (?v. (bir_eval_exp e env = SOME v) /\ (type_of_bir_val v = ty)))``,
+ ``!ext_map ext_st env e ty. (type_of_bir_exp ext_map e = SOME ty) ==>
+              ((bir_eval_exp ext_map e env ext_st = NONE) \/
+               (?v. (bir_eval_exp ext_map e env ext_st = SOME v) /\ (type_of_bir_val v = ty)))``,
 
-GEN_TAC >>
+NTAC 3 GEN_TAC >>
 Induct >> (
   SIMP_TAC (list_ss++bir_val_ss) [bir_eval_exp_def, type_of_bir_exp_def,
      type_of_bir_val_def] >>
@@ -102,7 +108,7 @@ Induct >> (
   FULL_SIMP_TAC (std_ss++bir_val_ss) [type_of_bir_val_EQ_ELIMS, bir_eval_memeq_REWRS,
     type_of_bir_val_def, BType_Bool_def, type_of_bool2b]
 ) >- (
-  Cases_on `bir_eval_exp e env = NONE` >- (
+  Cases_on `bir_eval_exp ext_map e env ext_st = NONE` >- (
     ASM_SIMP_TAC std_ss [bir_eval_ifthenelse_REWRS]
   ) >>
   FULL_SIMP_TAC std_ss [bir_eval_ifthenelse_REWRS, bir_type_is_Imm_def] >> 
@@ -110,9 +116,16 @@ Induct >> (
     FULL_SIMP_TAC (std_ss++bir_val_ss) [type_of_bir_val_EQ_ELIMS, bir_eval_ifthenelse_REWRS,
       BType_Bool_def, type_of_bir_val_def] >>
     CASE_TAC
-  ) >>
+  ) >> (
   FULL_SIMP_TAC (std_ss++bir_val_ss) [type_of_bir_val_EQ_ELIMS, bir_eval_ifthenelse_REWRS,
     BType_Bool_def, type_of_bir_val_def, type_of_bir_imm_def]
+  )
+) >- (
+  fs[bir_eval_extget_def] >>
+  rpt strip_tac >>
+  Cases_on `FLOOKUP (FST ext_map) s` >> (
+    fs []
+  )
 ) >- (
   FULL_SIMP_TAC std_ss [bir_eval_load_NONE_REWRS] >>
   FULL_SIMP_TAC std_ss [type_of_bir_val_EQ_ELIMS, bir_eval_load_def] >>
@@ -127,44 +140,47 @@ Induct >> (
 
 
 val type_of_bir_exp_EQ_SOME_REWRS = store_thm ("type_of_bir_exp_EQ_SOME_REWRS",``
-  (!i ty. (type_of_bir_exp (BExp_Const i) = SOME ty) <=> (ty = BType_Imm (type_of_bir_imm i))) /\
+  (!ext_map i ty. (type_of_bir_exp ext_map (BExp_Const i) = SOME ty) <=> (ty = BType_Imm (type_of_bir_imm i))) /\
 
-  (!aty vty mmap ty. (type_of_bir_exp (BExp_MemConst aty vty mmap) = SOME ty) <=> (ty = BType_Mem aty vty)) /\
+  (!ext_map aty vty mmap ty. (type_of_bir_exp ext_map (BExp_MemConst aty vty mmap) = SOME ty) <=> (ty = BType_Mem aty vty)) /\
 
-  (!v ty. (type_of_bir_exp (BExp_Den v) = SOME ty) <=> (ty = bir_var_type v)) /\
+  (!ext_map v ty. (type_of_bir_exp ext_map (BExp_Den v) = SOME ty) <=> (ty = bir_var_type v)) /\
 
-  (!ct e ty ty'. (type_of_bir_exp (BExp_Cast ct e ty') = SOME ty) <=> (
-     (ty = BType_Imm ty') /\ (?it. (type_of_bir_exp e = SOME (BType_Imm it))))) /\
+  (!ext_map ct e ty ty'. (type_of_bir_exp ext_map (BExp_Cast ct e ty') = SOME ty) <=> (
+     (ty = BType_Imm ty') /\ (?it. (type_of_bir_exp ext_map e = SOME (BType_Imm it))))) /\
 
-  (!et e ty. (type_of_bir_exp (BExp_UnaryExp et e) = SOME ty) <=> (
-     (bir_type_is_Imm ty) /\ (type_of_bir_exp e = SOME ty))) /\
+  (!ext_map et e ty. (type_of_bir_exp ext_map (BExp_UnaryExp et e) = SOME ty) <=> (
+     (bir_type_is_Imm ty) /\ (type_of_bir_exp ext_map e = SOME ty))) /\
 
-  (!et e1 e2 ty. (type_of_bir_exp (BExp_BinExp et e1 e2) = SOME ty) <=> (
-     (bir_type_is_Imm ty) /\ (type_of_bir_exp e1 = SOME ty) /\ (type_of_bir_exp e2 = SOME ty))) /\
+  (!ext_map et e1 e2 ty. (type_of_bir_exp ext_map (BExp_BinExp et e1 e2) = SOME ty) <=> (
+     (bir_type_is_Imm ty) /\ (type_of_bir_exp ext_map e1 = SOME ty) /\ (type_of_bir_exp ext_map e2 = SOME ty))) /\
 
-  (!pt e1 e2 ty. (type_of_bir_exp (BExp_BinPred pt e1 e2) = SOME ty) <=> (
-     (ty = BType_Bool) /\ (?it. (type_of_bir_exp e1 = SOME (BType_Imm it)) /\
-                              (type_of_bir_exp e2 = SOME (BType_Imm it))))) /\
+  (!ext_map pt e1 e2 ty. (type_of_bir_exp ext_map (BExp_BinPred pt e1 e2) = SOME ty) <=> (
+     (ty = BType_Bool) /\ (?it. (type_of_bir_exp ext_map e1 = SOME (BType_Imm it)) /\
+                              (type_of_bir_exp ext_map e2 = SOME (BType_Imm it))))) /\
 
-  (!me1 me2 ty. (type_of_bir_exp (BExp_MemEq me1 me2) = SOME ty) <=> (
-     ?at vt. (ty = BType_Bool) /\ (type_of_bir_exp me1 = SOME (BType_Mem at vt)) /\ (type_of_bir_exp me2 = type_of_bir_exp me1))) /\
+  (!ext_map me1 me2 ty. (type_of_bir_exp ext_map (BExp_MemEq me1 me2) = SOME ty) <=> (
+     ?at vt. (ty = BType_Bool) /\ (type_of_bir_exp ext_map me1 = SOME (BType_Mem at vt)) /\ (type_of_bir_exp ext_map me2 = type_of_bir_exp ext_map me1))) /\
 
-  (!ce e1 e2 ty. (type_of_bir_exp (BExp_IfThenElse ce e1 e2) = SOME ty) <=> (
-     (type_of_bir_exp ce = SOME BType_Bool) /\
-     (type_of_bir_exp e1 = SOME ty) /\
-     (type_of_bir_exp e2 = SOME ty))) /\
+  (!ext_map ce e1 e2 ty. (type_of_bir_exp ext_map (BExp_IfThenElse ce e1 e2) = SOME ty) <=> (
+     (type_of_bir_exp ext_map ce = SOME BType_Bool) /\
+     (type_of_bir_exp ext_map e1 = SOME ty) /\
+     (type_of_bir_exp ext_map e2 = SOME ty))) /\
 
-  (!rty ty ae en me. (type_of_bir_exp (BExp_Load me ae en rty) = SOME ty) <=> (
-     (ty = BType_Imm rty) /\ (?at vt. (type_of_bir_exp me = SOME (BType_Mem at vt)) /\
-                            (type_of_bir_exp ae = SOME (BType_Imm at)) /\
+  (!ext_map ext_name ty ty'. (type_of_bir_exp ext_map (BExp_ExtGet ext_name ty) = SOME ty') <=> (
+     ty = ty' /\ (?v. FLOOKUP (FST ext_map) ext_name = SOME v /\ type_of_bir_val v = ty))) /\
+
+  (!ext_map rty ty ae en me. (type_of_bir_exp ext_map (BExp_Load me ae en rty) = SOME ty) <=> (
+     (ty = BType_Imm rty) /\ (?at vt. (type_of_bir_exp ext_map me = SOME (BType_Mem at vt)) /\
+                            (type_of_bir_exp ext_map ae = SOME (BType_Imm at)) /\
                             (if en = BEnd_NoEndian then (vt = rty) else
                                   (bir_number_of_mem_splits vt rty at <> NONE))))) /\
 
-  (!ty ae en me v. (type_of_bir_exp (BExp_Store me ae en v) = SOME ty) <=> (
+  (!ext_map ty ae en me v. (type_of_bir_exp ext_map (BExp_Store me ae en v) = SOME ty) <=> (
      ?at vt rty. (ty = BType_Mem at vt) /\
-             (type_of_bir_exp me = SOME (BType_Mem at vt)) /\
-             (type_of_bir_exp ae = SOME (BType_Imm at)) /\
-             (type_of_bir_exp v = SOME (BType_Imm rty)) /\
+             (type_of_bir_exp ext_map me = SOME (BType_Mem at vt)) /\
+             (type_of_bir_exp ext_map ae = SOME (BType_Imm at)) /\
+             (type_of_bir_exp ext_map v = SOME (BType_Imm rty)) /\
              (if en = BEnd_NoEndian then (vt = rty) else
                                   (bir_number_of_mem_splits vt rty at <> NONE))))
 ``,
@@ -196,15 +212,17 @@ REPEAT CONJ_TAC >> (
   REPEAT GEN_TAC >> REPEAT CASE_TAC >> METIS_TAC[]
 ) >- (
   REPEAT GEN_TAC >> REPEAT CASE_TAC >> METIS_TAC[]
+) >- (
+  REPEAT GEN_TAC >> REPEAT CASE_TAC >> METIS_TAC[]
 ));
 
 
 val bir_eval_exp_IS_SOME_IMPLIES_TYPE =
   store_thm("bir_eval_exp_IS_SOME_IMPLIES_TYPE",
-  ``!env e va ty.
-    (bir_eval_exp e env = SOME va) ==>
+  ``!ext_map env ext_st e va ty.
+    (bir_eval_exp ext_map e env ext_st = SOME va) ==>
     (type_of_bir_val va = ty) ==>
-    (type_of_bir_exp e = SOME ty)``,
+    (type_of_bir_exp ext_map e = SOME ty)``,
 
 Induct_on `e` >> (
   REPEAT STRIP_TAC >>
@@ -222,7 +240,7 @@ Induct_on `e` >> (
   FULL_SIMP_TAC std_ss [],
 
   (* Cast *)
-  Cases_on `bir_eval_exp e env` >| [
+  Cases_on `bir_eval_exp ext_map e env ext_st` >| [
     FULL_SIMP_TAC std_ss [bir_eval_cast_def],
 
     Cases_on `x` >> (
@@ -233,7 +251,7 @@ Induct_on `e` >> (
   ],
 
   (* UnaryExp *)
-  Cases_on `bir_eval_exp e env` >| [
+  Cases_on `bir_eval_exp ext_map e env ext_st` >| [
     FULL_SIMP_TAC std_ss [bir_eval_unary_exp_def],
 
     Cases_on `x` >> (
@@ -244,7 +262,7 @@ Induct_on `e` >> (
   ],
 
   (* BinExp *)
-  Cases_on `bir_eval_exp e env` >> Cases_on `bir_eval_exp e' env` >> (
+  Cases_on `bir_eval_exp ext_map e env ext_st` >> Cases_on `bir_eval_exp ext_map e' env ext_st` >> (
     FULL_SIMP_TAC std_ss [bir_eval_bin_exp_REWRS]
   ) >>
   Cases_on `x` >> Cases_on `x'` >> (
@@ -254,7 +272,7 @@ Induct_on `e` >> (
 	     NOT_NONE_SOME, bir_type_is_Imm_def],
 
   (* BinPred *)
-  Cases_on `bir_eval_exp e env` >> Cases_on `bir_eval_exp e' env` >> (
+  Cases_on `bir_eval_exp ext_map e env ext_st` >> Cases_on `bir_eval_exp ext_map e' env ext_st` >> (
     FULL_SIMP_TAC std_ss [bir_eval_bin_pred_REWRS]
   ) >>
   Cases_on `x` >> Cases_on `x'` >> (
@@ -264,7 +282,7 @@ Induct_on `e` >> (
              bool2b_def, BType_Bool_def, type_of_bool2b],
 
   (* MemEq *)
-  Cases_on `bir_eval_exp e env` >> Cases_on `bir_eval_exp e' env` >> (
+  Cases_on `bir_eval_exp ext_map e env ext_st` >> Cases_on `bir_eval_exp ext_map e' env ext_st` >> (
     FULL_SIMP_TAC std_ss [bir_eval_memeq_REWRS]
   ) >>
   Cases_on `x` >> Cases_on `x'` >> (
@@ -274,8 +292,8 @@ Induct_on `e` >> (
              bool2b_def, BType_Bool_def, type_of_bool2b],
 
   (* IfThenElse *)
-  Cases_on `bir_eval_exp e env` >> Cases_on `bir_eval_exp e' env` >>
-    Cases_on `bir_eval_exp e'' env` >> (
+  Cases_on `bir_eval_exp ext_map e env ext_st` >> Cases_on `bir_eval_exp ext_map e' env ext_st` >>
+    Cases_on `bir_eval_exp ext_map e'' env ext_st` >> (
     FULL_SIMP_TAC std_ss [bir_eval_ifthenelse_REWRS]
   ) >>
   Cases_on `x` >> Cases_on `x'` >> Cases_on `x''` >> (
@@ -288,8 +306,14 @@ Induct_on `e` >> (
 	       bool2b_def, BType_Bool_def, type_of_bool2b]
   ),
 
+  (* ExtGet *)
+  fs [bir_eval_extget_def] >>
+  Cases_on `FLOOKUP (FST ext_map) s` >> (
+    gvs[]
+  ),
+
   (* Load *)
-  Cases_on `bir_eval_exp e env` >> Cases_on `bir_eval_exp e' env` >> (
+  Cases_on `bir_eval_exp ext_map e env ext_st` >> Cases_on `bir_eval_exp ext_map e' env ext_st` >> (
     FULL_SIMP_TAC std_ss [bir_eval_load_NONE_REWRS]
   ) >>
   Cases_on `x` >> Cases_on `x'` >> (
@@ -320,8 +344,8 @@ Induct_on `e` >> (
   ),
 
   (* Store *)
-  Cases_on `bir_eval_exp e env` >> Cases_on `bir_eval_exp e' env` >>
-    Cases_on `bir_eval_exp e'' env` >> (
+  Cases_on `bir_eval_exp ext_map e env ext_st` >> Cases_on `bir_eval_exp ext_map e' env ext_st` >>
+    Cases_on `bir_eval_exp ext_map e'' env ext_st` >> (
     FULL_SIMP_TAC std_ss [bir_eval_store_NONE_REWRS]
   ) >>
   Cases_on `x` >> Cases_on `x'` >> Cases_on `x''` >> (
@@ -348,46 +372,50 @@ Induct_on `e` >> (
 
 
 val type_of_bir_exp_EQ_NONE_REWRS = store_thm ("type_of_bir_exp_EQ_NONE_REWRS",``
-  (!i. ~(type_of_bir_exp (BExp_Const i) = NONE)) /\
+  (!ext_map i. ~(type_of_bir_exp ext_map (BExp_Const i) = NONE)) /\
 
-  (!aty vty mmap. ~(type_of_bir_exp (BExp_MemConst aty vty mmap) = NONE)) /\
+  (!ext_map aty vty mmap. ~(type_of_bir_exp ext_map (BExp_MemConst aty vty mmap) = NONE)) /\
 
-  (!v. ~(type_of_bir_exp (BExp_Den v) = NONE)) /\
+  (!ext_map v. ~(type_of_bir_exp ext_map (BExp_Den v) = NONE)) /\
 
-  (!ct e ty ty'. (type_of_bir_exp (BExp_Cast ct e ty') = NONE) <=> (
-     (!ity. (type_of_bir_exp e <> SOME (BType_Imm ity))))) /\
+  (!ext_map ct e ty ty'. (type_of_bir_exp ext_map (BExp_Cast ct e ty') = NONE) <=> (
+     (!ity. (type_of_bir_exp ext_map e <> SOME (BType_Imm ity))))) /\
 
-  (!et e. (type_of_bir_exp (BExp_UnaryExp et e) = NONE) <=> (
-     (!ity. type_of_bir_exp e <> SOME (BType_Imm ity)))) /\
+  (!ext_map et e. (type_of_bir_exp ext_map (BExp_UnaryExp et e) = NONE) <=> (
+     (!ity. type_of_bir_exp ext_map e <> SOME (BType_Imm ity)))) /\
 
-  (!et e1 e2. (type_of_bir_exp (BExp_BinExp et e1 e2) = NONE) <=> !ity.
-     (type_of_bir_exp e1 <> SOME (BType_Imm ity)) \/
-     (type_of_bir_exp e2 <> SOME (BType_Imm ity))) /\
+  (!ext_map et e1 e2. (type_of_bir_exp ext_map (BExp_BinExp et e1 e2) = NONE) <=> !ity.
+     (type_of_bir_exp ext_map e1 <> SOME (BType_Imm ity)) \/
+     (type_of_bir_exp ext_map e2 <> SOME (BType_Imm ity))) /\
 
-  (!pt e1 e2. (type_of_bir_exp (BExp_BinPred pt e1 e2) = NONE) <=> !ity.
-     (type_of_bir_exp e1 <> SOME (BType_Imm ity)) \/
-     (type_of_bir_exp e2 <> SOME (BType_Imm ity))) /\
+  (!ext_map pt e1 e2. (type_of_bir_exp ext_map (BExp_BinPred pt e1 e2) = NONE) <=> !ity.
+     (type_of_bir_exp ext_map e1 <> SOME (BType_Imm ity)) \/
+     (type_of_bir_exp ext_map e2 <> SOME (BType_Imm ity))) /\
 
-  (!me1 me2. (type_of_bir_exp (BExp_MemEq me1 me2) = NONE) <=> !at vt.
-     (type_of_bir_exp me1 <> SOME (BType_Mem at vt)) \/
-     (type_of_bir_exp me2 <> SOME (BType_Mem at vt))) /\
+  (!ext_map me1 me2. (type_of_bir_exp ext_map (BExp_MemEq me1 me2) = NONE) <=> !at vt.
+     (type_of_bir_exp ext_map me1 <> SOME (BType_Mem at vt)) \/
+     (type_of_bir_exp ext_map me2 <> SOME (BType_Mem at vt))) /\
 
-  (!ce e1 e2 ty. (type_of_bir_exp (BExp_IfThenElse ce e1 e2) = NONE) <=> (
-     (type_of_bir_exp ce <> SOME BType_Bool) \/
-     (type_of_bir_exp e1 = NONE) \/
-     (type_of_bir_exp e2 <> type_of_bir_exp e1))) /\
+  (!ext_map ce e1 e2 ty. (type_of_bir_exp ext_map (BExp_IfThenElse ce e1 e2) = NONE) <=> (
+     (type_of_bir_exp ext_map ce <> SOME BType_Bool) \/
+     (type_of_bir_exp ext_map e1 = NONE) \/
+     (type_of_bir_exp ext_map e2 <> type_of_bir_exp ext_map e1))) /\
 
-  (!rty ty ae en me. (type_of_bir_exp (BExp_Load me ae en rty) = NONE) <=> (
-     (!at vt. (type_of_bir_exp me = SOME (BType_Mem at vt)) /\
-              (type_of_bir_exp ae = SOME (BType_Imm at)) ==>
+  (!ext_map en ty. (type_of_bir_exp ext_map (BExp_ExtGet en ty) = NONE) <=> (
+     (FLOOKUP (FST ext_map) en = NONE) \/
+     (?v. FLOOKUP (FST ext_map) en = SOME v /\ type_of_bir_val v <> ty))) /\
+
+  (!ext_map rty ty ae en me. (type_of_bir_exp ext_map (BExp_Load me ae en rty) = NONE) <=> (
+     (!at vt. (type_of_bir_exp ext_map me = SOME (BType_Mem at vt)) /\
+              (type_of_bir_exp ext_map ae = SOME (BType_Imm at)) ==>
               (if en = BEnd_NoEndian then (vt <> rty) else
                    (bir_number_of_mem_splits vt rty at = NONE))))) /\
 
-  (!ty ae en me v. (type_of_bir_exp (BExp_Store me ae en v) = NONE) <=> (
+  (!ext_map ty ae en me v. (type_of_bir_exp ext_map (BExp_Store me ae en v) = NONE) <=> (
      !at vt rty.
-             (type_of_bir_exp me = SOME (BType_Mem at vt)) /\
-             (type_of_bir_exp ae = SOME (BType_Imm at)) /\
-             (type_of_bir_exp v = SOME (BType_Imm rty)) ==>
+             (type_of_bir_exp ext_map me = SOME (BType_Mem at vt)) /\
+             (type_of_bir_exp ext_map ae = SOME (BType_Imm at)) /\
+             (type_of_bir_exp ext_map v = SOME (BType_Imm rty)) ==>
              (if en = BEnd_NoEndian then (vt <> rty) else
                                   (bir_number_of_mem_splits vt rty at = NONE))))
 ``,
@@ -421,18 +449,20 @@ REPEAT CONJ_TAC >> (
   REPEAT GEN_TAC >> REPEAT CASE_TAC >> METIS_TAC[]
 ) >- (
   REPEAT GEN_TAC >> REPEAT CASE_TAC >> METIS_TAC[]
+) >- (
+  REPEAT GEN_TAC >> REPEAT CASE_TAC >> METIS_TAC[]
 ));
 
 
 val type_of_bir_exp_NOT_SOME_Imm = prove(
-  ``!ex env. 
-    (!ity. type_of_bir_exp ex <> SOME (BType_Imm ity)) ==>
-    (?aty vty. (type_of_bir_exp ex = SOME (BType_Mem aty vty)) \/
-     (type_of_bir_exp ex = NONE)
+  ``!ext_map ex env. 
+    (!ity. type_of_bir_exp ext_map ex <> SOME (BType_Imm ity)) ==>
+    (?aty vty. (type_of_bir_exp ext_map ex = SOME (BType_Mem aty vty)) \/
+     (type_of_bir_exp ext_map ex = NONE)
     )``,
 
 REPEAT STRIP_TAC >>
-Cases_on `type_of_bir_exp ex` >> (
+Cases_on `type_of_bir_exp ext_map ex` >> (
   FULL_SIMP_TAC (std_ss) []
 ) >>
 Cases_on `x` >> (
@@ -441,26 +471,26 @@ Cases_on `x` >> (
 );
 
 val type_of_2bir_exp_NOT_SOME_Imm = prove(
-  ``!ex ex'. 
+  ``!ext_map ex ex'. 
     (!ity.
-     type_of_bir_exp ex <> SOME (BType_Imm ity) \/
-     type_of_bir_exp ex' <> SOME (BType_Imm ity)) ==>
-    ((?aty vty. type_of_bir_exp ex = SOME (BType_Mem aty vty)) \/
-     (type_of_bir_exp ex = NONE) \/
-     (?aty vty. type_of_bir_exp ex' = SOME (BType_Mem aty vty)) \/
-     (type_of_bir_exp ex' = NONE) \/
+     type_of_bir_exp ext_map ex <> SOME (BType_Imm ity) \/
+     type_of_bir_exp ext_map ex' <> SOME (BType_Imm ity)) ==>
+    ((?aty vty. type_of_bir_exp ext_map ex = SOME (BType_Mem aty vty)) \/
+     (type_of_bir_exp ext_map ex = NONE) \/
+     (?aty vty. type_of_bir_exp ext_map ex' = SOME (BType_Mem aty vty)) \/
+     (type_of_bir_exp ext_map ex' = NONE) \/
      (?ity' ity''.
-      (type_of_bir_exp ex = SOME (BType_Imm ity')) /\
-      (type_of_bir_exp ex' = SOME (BType_Imm ity'')) /\
+      (type_of_bir_exp ext_map ex = SOME (BType_Imm ity')) /\
+      (type_of_bir_exp ext_map ex' = SOME (BType_Imm ity'')) /\
       (ity' <> ity'')
      )
     )``,
 
 REPEAT STRIP_TAC >>
-Cases_on `type_of_bir_exp ex` >> (
+Cases_on `type_of_bir_exp ext_map ex` >> (
   FULL_SIMP_TAC std_ss []
 ) >>
-Cases_on `type_of_bir_exp ex'` >> (
+Cases_on `type_of_bir_exp ext_map ex'` >> (
   FULL_SIMP_TAC std_ss []
 ) >>
 Cases_on `x` >> Cases_on `x'` >> (
@@ -469,9 +499,9 @@ Cases_on `x` >> Cases_on `x'` >> (
 );
 
 val bir_type_of_bir_exp_NONE = store_thm("bir_type_of_bir_exp_NONE",
-  ``!ex env.
-    (type_of_bir_exp ex = NONE) ==>
-    (bir_eval_exp ex env = NONE)``,
+  ``!ext_map ex env ext_st.
+    (type_of_bir_exp ext_map ex = NONE) ==>
+    (bir_eval_exp ext_map ex env ext_st = NONE)``,
 
 REPEAT STRIP_TAC >>
 Induct_on `ex` >> (
@@ -484,7 +514,7 @@ Induct_on `ex` >> (
   ) >>
   (* The memory remains... *)
   IMP_RES_TAC type_of_bir_exp_THM >>
-  QSPECL_X_ASSUM ``!env. _`` [`env`] >>
+  QSPECL_X_ASSUM ``!ext_st env. _`` [`ext_st`, `env`] >>
   FULL_SIMP_TAC std_ss [bir_eval_cast_REWRS] >>
   Cases_on `v` >> (
     FULL_SIMP_TAC (std_ss++bir_type_ss) [bir_eval_cast_REWRS, type_of_bir_val_def]
@@ -495,7 +525,7 @@ Induct_on `ex` >> (
     FULL_SIMP_TAC std_ss [bir_eval_unary_exp_REWRS]
   ) >>
   IMP_RES_TAC type_of_bir_exp_THM >>
-  QSPECL_X_ASSUM ``!env. _`` [`env`] >>
+  QSPECL_X_ASSUM ``!ext_st env. _`` [`ext_st`, `env`] >>
   FULL_SIMP_TAC std_ss [bir_eval_unary_exp_REWRS] >>
   Cases_on `v` >> (
     FULL_SIMP_TAC (std_ss++bir_type_ss) [bir_eval_unary_exp_REWRS, type_of_bir_val_def]
@@ -508,8 +538,8 @@ Induct_on `ex` >> (
     IMP_RES_TAC type_of_bir_exp_THM
   ) >> (
     (* 3 cases, two of which are proved by the below: *)
-    QSPECL_X_ASSUM ``!env. _`` [`env`] >>
-    TRY (QSPECL_X_ASSUM ``!env. _`` [`env`]) >>
+    QSPECL_X_ASSUM ``!ext_st env. _`` [`ext_st`, `env`] >>
+    TRY (QSPECL_X_ASSUM ``!ext_st env. _`` [`ext_st`, `env`]) >>
     FULL_SIMP_TAC std_ss [bir_eval_bin_exp_REWRS] >>
     Cases_on `v` >> (
       FULL_SIMP_TAC (std_ss++bir_type_ss) [bir_eval_bin_exp_REWRS, type_of_bir_val_def]
@@ -526,8 +556,8 @@ Induct_on `ex` >> (
   ) >> (
     IMP_RES_TAC type_of_bir_exp_THM
   ) >> (
-    QSPECL_X_ASSUM ``!env. _`` [`env`] >>
-    TRY (QSPECL_X_ASSUM ``!env. _`` [`env`]) >>
+    QSPECL_X_ASSUM ``!ext_st env. _`` [`ext_st`, `env`] >>
+    TRY (QSPECL_X_ASSUM ``!ext_st env. _`` [`ext_st`, `env`]) >>
     FULL_SIMP_TAC std_ss [bir_eval_bin_pred_REWRS] >>
     Cases_on `v` >> (
       FULL_SIMP_TAC (std_ss++bir_type_ss) [bir_eval_bin_pred_REWRS, type_of_bir_val_def]
@@ -538,14 +568,14 @@ Induct_on `ex` >> (
   ),
 
   (* MemEq *)
-  Cases_on `type_of_bir_exp ex` >> Cases_on `type_of_bir_exp ex'` >> (
+  Cases_on `type_of_bir_exp ext_map ex` >> Cases_on `type_of_bir_exp ext_map ex'` >> (
     FULL_SIMP_TAC std_ss [bir_eval_memeq_REWRS]
   ) >>
   IMP_RES_TAC type_of_bir_exp_THM >>
   Cases_on `x` >> Cases_on `x'` >> (
     FULL_SIMP_TAC (std_ss++bir_type_ss) [] >>
-    REPEAT (QSPECL_X_ASSUM ``!env. _`` [`env`]) >>
-    FULL_SIMP_TAC (std_ss) [bir_eval_memeq_REWRS]
+    REPEAT (QSPECL_X_ASSUM ``!ext_st env. _`` [`ext_st`, `env`]) >>
+    FULL_SIMP_TAC std_ss [bir_eval_memeq_REWRS]
   ) >> (
     Cases_on `v` >> (
       FULL_SIMP_TAC (std_ss++bir_type_ss) [bir_eval_memeq_REWRS, type_of_bir_val_def]
@@ -557,33 +587,39 @@ Induct_on `ex` >> (
 
   (* IfThenElse condition *)
   FULL_SIMP_TAC std_ss [BType_Bool_def] >>
-  Cases_on `type_of_bir_exp ex` >> (
+  Cases_on `type_of_bir_exp ext_map ex` >> (
     FULL_SIMP_TAC (std_ss++bir_type_ss) [bir_eval_ifthenelse_REWRS]
   ) >>
   IMP_RES_TAC type_of_bir_exp_THM >>
-  QSPECL_X_ASSUM ``!env. _`` [`env`] >>
+  QSPECL_X_ASSUM ``!ext_st env. _`` [`ext_st`, `env`] >>
   FULL_SIMP_TAC std_ss [bir_eval_ifthenelse_REWRS, bir_eval_ifthenelse_REWRS_NONE],
 
   (* IfThenElse second argument NONE *)
   FULL_SIMP_TAC std_ss [bir_eval_ifthenelse_REWRS],
 
   (* IfThenElse type mismatch *)
-  Cases_on `type_of_bir_exp ex'` >> (
+  Cases_on `type_of_bir_exp ext_map ex'` >> (
     FULL_SIMP_TAC std_ss [bir_eval_ifthenelse_REWRS]
   ) >>
-  Cases_on `type_of_bir_exp ex''` >> (
+  Cases_on `type_of_bir_exp ext_map ex''` >> (
     FULL_SIMP_TAC std_ss [bir_eval_ifthenelse_REWRS]
   ) >>
   IMP_RES_TAC type_of_bir_exp_THM >>
-  REPEAT (QSPECL_X_ASSUM ``!env. _`` [`env`]) >>
+  REPEAT (QSPECL_X_ASSUM ``!ext_st env. _`` [`ext_st`, `env`]) >>
   FULL_SIMP_TAC std_ss [bir_eval_ifthenelse_REWRS, bir_eval_ifthenelse_REWRS_NONE],
 
+  (* ExtGet - NONE *)
+  fs[bir_eval_extget_def],
+
+  (* ExtGet - SOME *)
+  fs[bir_eval_extget_def],
+
   (* Load *)
-  Cases_on `type_of_bir_exp ex` >> Cases_on `type_of_bir_exp ex'` >> (
+  Cases_on `type_of_bir_exp ext_map ex` >> Cases_on `type_of_bir_exp ext_map ex'` >> (
     FULL_SIMP_TAC std_ss [bir_eval_load_NONE_REWRS]
   ) >>
   IMP_RES_TAC type_of_bir_exp_THM >>
-  NTAC 2 (QSPECL_X_ASSUM ``!env. _`` [`env`]) >>
+  NTAC 2 (QSPECL_X_ASSUM ``!ext_st env. _`` [`ext_st`, `env`]) >>
   FULL_SIMP_TAC std_ss [bir_eval_load_NONE_REWRS] >>
   Cases_on `v` >> Cases_on `v'` >> (
     FULL_SIMP_TAC std_ss [bir_eval_load_NONE_REWRS]
@@ -602,12 +638,12 @@ Induct_on `ex` >> (
   ),
 
   (* Store *)
-  Cases_on `type_of_bir_exp ex` >> Cases_on `type_of_bir_exp ex'` >>
-    Cases_on `type_of_bir_exp ex''` >> (
+  Cases_on `type_of_bir_exp ext_map ex` >> Cases_on `type_of_bir_exp ext_map ex'` >>
+    Cases_on `type_of_bir_exp ext_map ex''` >> (
     FULL_SIMP_TAC std_ss [bir_eval_store_NONE_REWRS]
   ) >>
   IMP_RES_TAC type_of_bir_exp_THM >>
-  NTAC 3 (QSPECL_X_ASSUM ``!env. _`` [`env`]) >>
+  NTAC 3 (QSPECL_X_ASSUM ``!ext_st env. _`` [`ext_st`, `env`]) >>
   FULL_SIMP_TAC std_ss [bir_eval_store_NONE_REWRS] >>
   Cases_on `v` >> Cases_on `v'` >> Cases_on `v''` >> (
     FULL_SIMP_TAC std_ss [bir_eval_store_NONE_REWRS]
@@ -642,16 +678,17 @@ val bir_vars_of_exp_def = Define `
   (bir_vars_of_exp (BExp_BinPred _ e1 e2) = (bir_vars_of_exp e1 UNION bir_vars_of_exp e2)) /\
   (bir_vars_of_exp (BExp_MemEq e1 e2) = (bir_vars_of_exp e1 UNION bir_vars_of_exp e2)) /\
   (bir_vars_of_exp (BExp_IfThenElse ec e1 e2) = (bir_vars_of_exp ec UNION bir_vars_of_exp e1 UNION bir_vars_of_exp e2)) /\
+  (bir_vars_of_exp (BExp_ExtGet en ty) = {}) /\
   (bir_vars_of_exp (BExp_Load me ae _ _) = (bir_vars_of_exp me UNION bir_vars_of_exp ae)) /\
   (bir_vars_of_exp (BExp_Store me ae _ ve) = (bir_vars_of_exp me UNION bir_vars_of_exp ae UNION bir_vars_of_exp ve))`;
 
 
 val bir_vars_of_exp_THM = store_thm ("bir_vars_of_exp_THM",
-``!env1 env2 e. (!v. v IN (bir_vars_of_exp e) ==>
+``!env1 env2 e ext_map ext_st. (!v. v IN (bir_vars_of_exp e) ==>
                      (bir_env_read v env1 = bir_env_read v env2)) ==>
-                (bir_eval_exp e env1 = bir_eval_exp e env2)``,
+                (bir_eval_exp ext_map e env1 ext_st = bir_eval_exp ext_map e env2 ext_st)``,
 
-GEN_TAC >> GEN_TAC >> Induct >> REPEAT STRIP_TAC >> (
+NTAC 2 GEN_TAC >> Induct >> REPEAT STRIP_TAC >> (
   FULL_SIMP_TAC std_ss [bir_vars_of_exp_def, pred_setTheory.IN_UNION,
     pred_setTheory.NOT_IN_EMPTY, pred_setTheory.IN_INSERT,
     bir_eval_exp_def]
@@ -659,8 +696,8 @@ GEN_TAC >> GEN_TAC >> Induct >> REPEAT STRIP_TAC >> (
 
 
 val bir_vars_of_exp_THM_EQ_FOR_VARS = store_thm ("bir_vars_of_exp_THM_EQ_FOR_VARS",
-``!env1 env2 e. (bir_env_EQ_FOR_VARS (bir_vars_of_exp e) env1 env2) ==>
-                (bir_eval_exp e env1 = bir_eval_exp e env2)``,
+``!ext_map env1 env2 e ext_st. (bir_env_EQ_FOR_VARS (bir_vars_of_exp e) env1 env2) ==>
+                (bir_eval_exp ext_map e env1 ext_st = bir_eval_exp ext_map e env2 ext_st)``,
 METIS_TAC[bir_vars_of_exp_THM, bir_env_EQ_FOR_VARS_read_IMPL]);
 
 
@@ -675,12 +712,12 @@ Induct >> (
 
 
 val type_of_bir_exp_THM_with_envty = store_thm ("type_of_bir_exp_THM_with_envty",
-  ``!env envty e ty. (type_of_bir_exp e = SOME ty) ==>
+  ``!ext_map env ext_st envty e ty. (type_of_bir_exp ext_map e = SOME ty) ==>
                      (bir_envty_includes_vs envty (bir_vars_of_exp e)) ==>
                      (bir_env_satisfies_envty env envty) ==>
-                     (?v. ((bir_eval_exp e env) = SOME v) /\ (type_of_bir_val v = ty))``,
+                     (?v. ((bir_eval_exp ext_map e env ext_st) = SOME v) /\ (type_of_bir_val v = ty))``,
 
-GEN_TAC >> GEN_TAC >> Induct >> (
+NTAC 4 GEN_TAC >> Induct >> (
   SIMP_TAC (std_ss++bir_val_ss) [bir_eval_exp_def, BType_Bool_def,
     type_of_bir_exp_EQ_SOME_REWRS, bir_vars_of_exp_def,
     bir_envty_includes_vs_UNION, bir_envty_includes_vs_INSERT,
@@ -704,6 +741,9 @@ GEN_TAC >> GEN_TAC >> Induct >> (
 ) >- (
   ASM_SIMP_TAC (std_ss++bir_val_ss) [bir_eval_ifthenelse_REWRS] >>
   METIS_TAC[]
+) >- (
+  fs[bir_eval_extget_def] >>
+  metis_tac[]
 ) >- (
   ASM_SIMP_TAC (std_ss++bir_val_ss) [bir_eval_load_BASIC_REWR] >>
   rename1 `bir_load_from_mem vt ity at mmap en (b2n i)` >>
@@ -732,9 +772,9 @@ GEN_TAC >> GEN_TAC >> Induct >> (
 (* TODO: move elsewhere *)
 open bir_env_oldTheory;
 val type_of_bir_exp_THM_with_init_vars = store_thm ("type_of_bir_exp_THM_with_init_vars",
-  ``!env e ty. (type_of_bir_exp e = SOME ty) ==>
+  ``!ext_map env e ty ext_st. (type_of_bir_exp ext_map e = SOME ty) ==>
                (bir_env_vars_are_initialised env (bir_vars_of_exp e)) ==>
-               (?va. (bir_eval_exp e env = SOME va) /\ (type_of_bir_val va = ty))``,
+               (?va. (bir_eval_exp ext_map e env ext_st = SOME va) /\ (type_of_bir_val va = ty))``,
   METIS_TAC [type_of_bir_exp_THM_with_envty, bir_env_vars_are_initialised_EQ_envty, bir_env_satisfies_envty_of_env]
 );
 
@@ -743,8 +783,8 @@ val type_of_bir_exp_THM_with_init_vars = store_thm ("type_of_bir_exp_THM_with_in
  * of expressions in assumptions *)
 val bir_eval_exp_IS_SOME_IMPLIES_INIT =
   store_thm("bir_eval_exp_IS_SOME_IMPLIES_INIT",
-  ``!env e va.
-    (bir_eval_exp e env = SOME va) ==>
+  ``!ext_map env e ext_st va.
+    (bir_eval_exp ext_map e env ext_st = SOME va) ==>
     bir_env_vars_are_initialised env (bir_vars_of_exp e)``,
 
 Induct_on `e` >> (
@@ -761,40 +801,40 @@ Induct_on `e` >> (
                         pred_setTheory.IN_SING, bir_env_oldTheory.bir_env_var_is_initialised_def],
 
   (* Cast *)
-  Cases_on `bir_eval_exp e env` >- (
+  Cases_on `bir_eval_exp ext_map e env ext_st` >- (
     FULL_SIMP_TAC std_ss [bir_eval_cast_REWRS]
   ) >>
   METIS_TAC [],
 
   (* UnaryExp *)
-  Cases_on `bir_eval_exp e env` >- (
+  Cases_on `bir_eval_exp ext_map e env ext_st` >- (
     FULL_SIMP_TAC std_ss [bir_eval_unary_exp_REWRS]
   ) >>
   METIS_TAC [],
 
   (* BinExp *)
-  Cases_on `bir_eval_exp e env` >- (
+  Cases_on `bir_eval_exp ext_map e env ext_st` >- (
     FULL_SIMP_TAC std_ss [bir_eval_bin_exp_REWRS]
   ) >>
-  Cases_on `bir_eval_exp e' env` >- (
+  Cases_on `bir_eval_exp ext_map e' env ext_st` >- (
     FULL_SIMP_TAC std_ss [bir_eval_bin_exp_REWRS]
   ) >>
   METIS_TAC [bir_env_oldTheory.bir_env_vars_are_initialised_UNION],
 
   (* BinPred *)
-  Cases_on `bir_eval_exp e env` >- (
+  Cases_on `bir_eval_exp ext_map e env ext_st` >- (
     FULL_SIMP_TAC std_ss [bir_eval_bin_pred_REWRS]
   ) >>
-  Cases_on `bir_eval_exp e' env` >- (
+  Cases_on `bir_eval_exp ext_map e' env ext_st` >- (
     FULL_SIMP_TAC std_ss [bir_eval_bin_pred_REWRS]
   ) >>
   METIS_TAC [bir_env_oldTheory.bir_env_vars_are_initialised_UNION],
 
   (* MemEq *)
-  Cases_on `bir_eval_exp e env` >- (
+  Cases_on `bir_eval_exp ext_map e env ext_st` >- (
     FULL_SIMP_TAC std_ss [bir_eval_memeq_REWRS]
   ) >>
-  Cases_on `bir_eval_exp e' env` >- (
+  Cases_on `bir_eval_exp ext_map e' env ext_st` >- (
     Cases_on `x` >> (
       FULL_SIMP_TAC std_ss [bir_eval_memeq_REWRS]
     )
@@ -802,22 +842,22 @@ Induct_on `e` >> (
   METIS_TAC [bir_env_oldTheory.bir_env_vars_are_initialised_UNION],
 
   (* IfThenElse *)
-  Cases_on `bir_eval_exp e env` >- (
+  Cases_on `bir_eval_exp ext_map e env ext_st` >- (
     FULL_SIMP_TAC std_ss [bir_eval_ifthenelse_REWRS]
   ) >>
-  Cases_on `bir_eval_exp e' env` >- (
+  Cases_on `bir_eval_exp ext_map e' env ext_st` >- (
     FULL_SIMP_TAC std_ss [bir_eval_ifthenelse_REWRS]
   ) >>
-  Cases_on `bir_eval_exp e'' env` >- (
+  Cases_on `bir_eval_exp ext_map e'' env ext_st` >- (
     FULL_SIMP_TAC std_ss [bir_eval_ifthenelse_REWRS]
   ) >>
   METIS_TAC [bir_env_oldTheory.bir_env_vars_are_initialised_UNION],
 
   (* Load *)
-  Cases_on `bir_eval_exp e env` >- (
+  Cases_on `bir_eval_exp ext_map e env ext_st` >- (
     FULL_SIMP_TAC std_ss [bir_eval_load_NONE_REWRS]
   ) >>
-  Cases_on `bir_eval_exp e' env` >- (
+  Cases_on `bir_eval_exp ext_map e' env ext_st` >- (
     Cases_on `x` >> (
       FULL_SIMP_TAC std_ss [bir_eval_load_NONE_REWRS]
     )
@@ -825,13 +865,13 @@ Induct_on `e` >> (
   METIS_TAC [bir_env_oldTheory.bir_env_vars_are_initialised_UNION],
 
   (* Store *)
-  Cases_on `bir_eval_exp e env` >- (
+  Cases_on `bir_eval_exp ext_map e env ext_st` >- (
     FULL_SIMP_TAC std_ss [bir_eval_store_NONE_REWRS]
   ) >>
-  Cases_on `bir_eval_exp e' env` >- (
+  Cases_on `bir_eval_exp ext_map e' env ext_st` >- (
     FULL_SIMP_TAC std_ss [bir_eval_store_NONE_REWRS]
   ) >>
-  Cases_on `bir_eval_exp e'' env` >- (
+  Cases_on `bir_eval_exp ext_map e'' env ext_st` >- (
     FULL_SIMP_TAC std_ss [bir_eval_store_NONE_REWRS]
   ) >>
   METIS_TAC [bir_env_oldTheory.bir_env_vars_are_initialised_UNION]
@@ -851,8 +891,8 @@ Induct_on `e` >> (
    More subtly, one needs also make sure that variables occuring in the expression
    are having consistent type annotations. This is expressed as follows: *)
 
-val bir_exp_is_well_typed_def = Define `bir_exp_is_well_typed e <=>
-  (IS_SOME (type_of_bir_exp e) /\
+val bir_exp_is_well_typed_def = Define `bir_exp_is_well_typed ext_map e <=>
+  (IS_SOME (type_of_bir_exp ext_map e) /\
    bir_vs_consistent (bir_vars_of_exp e))`
 
 
